proof/DSG.thy
@@ -1,0 +1,131 @@
+theory DSG
+  imports Main History
+begin
+
+section \<open>Transaction Dependencies\<close>
+
+text \<open>We begin by formalizing three types of dependencies between transactions: wr-depends,
+ww-depends, and rw-depends. The wr-depends relation captures the idea of a transaction t2 reading
+another transaction T1's write.\<close>
+
+definition wr_depends :: "history \<Rightarrow> atxn \<Rightarrow> atxn \<Rightarrow> bool" where
+"wr_depends h t1 t2 \<equiv> \<exists>w1 r2. (a_is_committed t1) \<and>
+                              (a_is_committed t2) \<and>
+                              (w1 \<in> ext_awrites t1) \<and>
+                              (r2 \<in> ext_areads t2) \<and>
+                              ((key w1) = (key r2)) \<and>
+                              ((post_version w1) = (pre_version r2))"
+
+text \<open>We say t1 ww-depends t2 if t2 overwrote t1--that is, if t1 installed
+some version v1 of k, and t2 wrote v2, such that v1 came immediately before v2 in the version order
+of k.\<close>
+
+definition ww_depends :: "history \<Rightarrow> atxn \<Rightarrow> atxn \<Rightarrow> bool" where
+"ww_depends h t1 t2 \<equiv> \<exists>w1 w2.
+  (a_is_committed t1) \<and>
+  (a_is_committed t2) \<and>
+  (w1 \<in> ext_awrites t1) \<and>
+  (w2 \<in> ext_awrites t2) \<and>
+  ((key w1) = (key w2)) \<and>
+  (is_next_in_history h (key w1) (apost_version w1) (apost_version w2))"
+
+lemma ww_depends_example: "ww_depends 
+  (History objs
+           {(ATxn [(AWrite x v0 a1 v1 [])] True),
+            (ATxn [(AWrite x v1 a2 v2 [])] True)}
+           {(KeyVersionOrder x [v0, v1, v2])})
+  (ATxn [(AWrite x v0 a1 v1 [])] True)
+  (ATxn [(AWrite x v1 a2 v2 [])] True)
+= True"
+  apply (simp add:ww_depends_def)
+  done
+
+text \<open>An rw-dependency is just like a ww-dependency, only transaction t1 *read* state just prior to
+t2's write.\<close>
+
+definition rw_depends :: "history \<Rightarrow> atxn \<Rightarrow> atxn \<Rightarrow> bool" where
+"rw_depends h t1 t2 \<equiv> \<exists>r1 w2.
+  (a_is_committed t1) \<and>
+  (a_is_committed t2) \<and>
+  (r1 \<in> ext_areads t1) \<and>
+  (w2 \<in> ext_awrites t2) \<and>
+  ((key r1) = (key w2)) \<and>
+  (is_next_in_history h (key r1) (apost_version r1) (apost_version w2))"
+
+section \<open>Direct Serialization Graphs\<close>
+
+text \<open>Now, we define a Direct Serialization Graph of a history as a graph where nodes are
+transactions in that history, and arcs are dependencies between them. We codify these three types of
+dependency with a type, and create a dependency type to wrap them. We call these aDeps for abstract
+dependencies; later, we'll define analogous observed dependencies.\<close>
+
+datatype depType = WR | WW | RW
+
+datatype adep = ADep atxn depType atxn
+
+primrec adep_head :: "adep \<Rightarrow> atxn" where
+"adep_head (ADep t _ _) = t"
+
+primrec adep_tail :: "adep \<Rightarrow> atxn" where
+"adep_tail (ADep _ _ t) = t"
+
+class dep_typed =
+  fixes dep_type :: "'a \<Rightarrow> depType"
+
+instantiation adep :: "dep_typed"
+begin
+primrec dep_type_adep :: "adep \<Rightarrow> depType" where
+"dep_type_adep (ADep _ t _) = t"
+instance ..
+end
+
+type_synonym dsg = "(atxn, adep) pre_digraph"
+
+text \<open>The DSG of a history is defined by mapping each dependency to an edge in the graph.\<close>
+
+definition dsg :: "history \<Rightarrow> dsg" where
+"dsg h \<equiv> \<lparr>verts = all_atxns h,
+          arcs  = ({(ADep t1 WR t2) | t1 t2. wr_depends h t1 t2} \<union>
+                   {(ADep t1 WW t2) | t1 t2. ww_depends h t1 t2} \<union>
+                   {(ADep t1 RW t2) | t1 t2. rw_depends h t1 t2}),
+          tail = adep_tail,
+          head = adep_head\<rparr>"
+
+
+text \<open>Now, we need to characterize a cycle in a DSG. TODO: I don't know how to use the definitions
+in the locales in Arc_Walk.thy, but I assume we should take advantage of them. Copy-pasting with
+slight mods for now.\<close>
+
+type_synonym 'a path = "'a list"
+
+text \<open>The list of vertices of a walk. The additional vertex argument is there to deal with the case
+of empty walks.\<close>
+
+primrec path_verts :: "('a,'b) pre_digraph \<Rightarrow> 'a \<Rightarrow> 'b path \<Rightarrow> 'a list" where
+    "path_verts G u [] = [u]"
+  | "path_verts G u (e # es) = tail G e # path_verts G (head G e) es"
+
+text \<open>
+  Tests whether a list of arcs is a consistent arc sequence,
+  i.e. a list of arcs, where the head G node of each arc is
+  the tail G node of the following arc.
+\<close>
+fun cas :: "('a, 'b) pre_digraph => 'a \<Rightarrow> 'b path \<Rightarrow> 'a \<Rightarrow> bool" where
+  "cas G u [] v = (u = v)" |
+  "cas G u (e # es) v = (tail G e = u \<and> cas G (head G e) es v)"
+
+definition path :: "('a,'b) pre_digraph \<Rightarrow> 'a \<Rightarrow> 'b path \<Rightarrow> 'a \<Rightarrow> bool" where
+  "path G u p v \<equiv> u \<in> verts G \<and> set p \<subseteq> arcs G \<and> cas G u p v"
+
+text \<open>Is the given path a cycle in the given graph?\<close>
+
+definition cycle :: "('a,'b) pre_digraph \<Rightarrow> 'b path \<Rightarrow> bool" where
+  "cycle G p \<equiv> \<exists>u. path G u p u \<and> distinct (tl (path_verts G u p)) \<and> p \<noteq> []"
+
+text \<open>We would like a cycle whose edges are all of the given set of dependency types.\<close>
+
+primrec path_dep_types :: "('a::dep_typed) path \<Rightarrow> depType set" where
+"path_dep_types []        = {}" |
+"path_dep_types (x # xs)  = (Set.insert (dep_type x) (path_dep_types xs))"
+
+end
